\documentclass{article}
\usepackage{amsmath}
\usepackage{gensymb}
\usepackage{nicefrac}
\usepackage{multirow}
\usepackage{graphicx}
\usepackage[mathscr]{euscript}
\usepackage[margin=4cm]{geometry}

\title{Swinging Atwood Machine}
\author{Michael Kister, Alli Behr}
\date{}

\begin{document}
\maketitle

\section*{Lagrangian Function}

\begin{gather*}
\mathscr{L} = \mathscr{L}(q_{1}, \ldots, q_{n}, \dot{q_{1}}, \ldots, \dot{q_{n}}, t) = T - U \\
\end{gather*}

\begin{gather*}
\frac{\partial \mathscr{L}}{\partial q_{i}} = \frac{d}{dt}\frac{\partial \mathscr{L}}{\partial \dot{q_{ix}}}
\end{gather*}

\begin{gather*}
p_{i} = \frac{\partial \mathscr{L}}{\partial \dot{q_{i}}}
\end{gather*}

\section*{Hamiltonian}

\begin{gather*}
\mathscr{H} = \sum_{i = 1}^{n}p_{i}\dot{q_{i}} - \mathscr{L}
\end{gather*}

\begin{gather*}
\mathscr{H} = \mathscr{H}(q_{1}, \ldots, q_{n}, p_{1}, \ldots, p_{n})
\end{gather*}

\begin{gather*}
\mathscr{H} = T + U
\end{gather*}

\begin{gather*}
\dot{q}_{i} = \frac{\partial \mathscr{H}}{\partial p_{i}} \qquad\text{and}\qquad \dot{p_{i}} = - \frac{\partial \mathscr{H}}{\partial q_{i}}
\end{gather*}

\section*{Swinging Atwood Machine}

\begin{align*}
T &= \frac{1}{2}m_{1}v_{1}^{2}+\frac{1}{2}m_{1}v_{2}^{2} \\
&= \frac{1}{2}m_{1}\left( \dot{r_{1}}^{2} + (r_{1}\dot{\theta_{1}})^{2} \right) \,+\, \frac{1}{2}m_{2}\left( \dot{r_{2}}^{2} + (r_{2}\dot{\theta_{2}})^{2} \right) \\
U &= m_{1} \, g \, \left[ r_{1} \, (1-\cos{\theta_{1}}) + (R - r_{1}) \right] \,+\, m_{2} \, g \, \left[ r_{2} \, (1-\cos{\theta_{2}}) + (R - r_{2})\right]
\end{align*}

\begin{align*}
r_{2} = R - r_{1} \qquad&\text{and}\qquad \dot{r_{2}} = -\dot{r_{1}} \\
\dot{\theta_{2}} = 0 \qquad&\text{and}\qquad \theta_{2} = 0
\end{align*}

\begin{gather*}
\mathscr{H} = \frac{1}{2}m_{1}\left( \dot{r_{1}}^{2} + (r_{1}\dot{\theta_{1}})^{2} \right) \,+\, \frac{1}{2}m_{2}\dot{r}_{1}^{2} \,-\, m_{1}\,g\,r_{1}\,\cos{\theta_{1}} \,+\, m_{2}\,g\,r_{1} \\
\text{or} \\
\mathscr{H} = \frac{1}{2}m_{1}\left( \dot{r}^{2} + (r\,\dot{\theta})^{2} \right) \,+\, \frac{1}{2}m_{2}\,\dot{r}^{2} \,-\, m_{1}\,g\,r\,\cos{\theta} \,+\, m_{2}\,g\,r
\end{gather*}

\begin{align*}
p_{r} = \frac{\partial \mathscr{L}}{\partial \dot{r}} &= \frac{\partial T}{\partial \dot{r}} \\
&= \frac{\partial}{\partial \dot{r}} \left( \frac{1}{2}m_{1}\left( \dot{r}^{2} + (r\,\dot{\theta})^{2} \right) \,+\, \frac{1}{2}m_{2}\,\dot{r}^{2} \right) \\
&= \dot{r}(m_{1} +m_{2}) \implies \\
\dot{r} &= \frac{p_{r}}{(m_{1}+m_{2})} \\
\\
&\text{and:} \\
\\
p_{\theta} = \frac{\partial \mathscr{L}}{\partial \dot{\theta}} &= \frac{\partial T}{\partial \dot{\theta}} \\
&= \frac{\partial}{\partial \dot{\theta}}\left( \frac{1}{2}m_{1}\left( \dot{r}^{2} + (r\,\dot{\theta})^{2} \right) \,+\, \frac{1}{2}m_{2}\,\dot{r}^{2} \right) \\
&= m_{1} \, r^{2} \, \dot{\theta} \implies \\
\dot{\theta} &= \frac{p_{\theta}}{m_{1}\,r^{2}}
\end{align*}

\begin{gather*}
\mathscr{H} = \frac{1}{2}m_{1}\left[ \left(\frac{p_{r}}{(m_{1}+m_{2})}\right)^{2} + \left(r\,\left(\frac{p_{\theta}}{m_{1}\,r^{2}}\right)\right)^{2} \right] \,+\, \frac{1}{2}m_{2}\,\left(\frac{p_{r}}{(m_{1}+m_{2})}\right)^{2} \,-\, m_{1}\,g\,r\,\cos{\theta} \,+\, m_{2}\,g\,r \\
\\
\text{which simplifies to:} \\
\\
\mathscr{H} = \frac{p_{r}^{2}}{2(m_{1}+m_{2})} \,+\, \frac{p_{\theta}^{2}}{2\,m_{1}\,r^{2}} \,+\, m_{2}\,g\,r \,-\, m_{1}\,g\,r\,\cos{\theta}
\end{gather*}

\begin{align*}
\dot{\theta} = \frac{\partial \mathscr{H}}{\partial p_{\theta}} = \frac{p_{\theta}}{m_{1}\,r^{2}} \qquad&\qquad\qquad \dot{p_{\theta}} = -\frac{\partial \mathscr{H}}{\partial \theta} = -m_{1}\,g\,r\,\sin{\theta} \\
\dot{r} = \frac{\partial \mathscr{H}}{\partial p_{r}} = \frac{p_{r}}{(m_{1}+m_{2})} \qquad&\qquad\qquad \dot{p_{r}} = -\frac{\partial \mathscr{H}}{\partial r} = \frac{p_{\theta}^{2}}{m_{1}\,r^{3}} \,-\, m_{2}\,g \,+\, m_{1}\,g\,\cos{\theta} \\
\end{align*}

\end{document}